moved LTS_functions to a new file and fixed f_out + ind_ioco

src/IOCO.v
@@ -1,38 +1,72 @@
 Require Import IOTS.
 Require Import LTS.
+Require Import LTS_functions.
 Require Import Bool BinPos BinNat PeanoNat Nnat.
 Require Import Coq.Lists.List.
 Require Import Coq.Lists.ListSet.
 Import Coq.Lists.List.ListNotations.
 Require Import String.
 
-Fixpoint out_labels (ll : set label) (l_u : set label) : set label := 
-match ll with
-| []      =>  []
-| h :: t  =>  if in_dec string_dec h l_u then set_add string_dec h (out_labels t l_u) 
-                                         else out_labels t l_u
-end.
+Inductive out_label : Type :=
+  | out_event : label -> out_label
+  | delta : out_label.
 
-Fixpoint in_labels (ll : set label) (l_i : set label) : set label := 
-match ll with
-| []      =>  []
-| h :: t  =>  if in_dec string_dec h l_i then set_add string_dec h (in_labels t l_i) 
-                                         else in_labels t l_i
-end.
-(*
-Fixpoint f_out (ls : set state) (p : s_IOLTS) : set label :=
-match ls with
-| []      =>  []
-| h :: t  =>  match out_labels (f_init h p.(T_del)) p.(Lu_del) with
-              | [] =>  set_union string_dec [delta] (f_out t p)
-              | a  =>  set_union string_dec a (f_out t p)
-              end
-end.
+Inductive ind_out_one_state : state -> set out_label -> s_IOLTS -> Prop :=
+  | out_one_state_r1 (s : state) (p : s_IOLTS) :
+      In s p.(Ts) -> ind_out_one_state s [delta] p
+  | out_one_state_r2 (s : state) (p : s_IOLTS) (so : set out_label) :
+      ~ In delta so ->
+      (forall (l : label) (s' : state),
+        In (out_event l) so <->
+        In l p.(iolts).(L_u) /\ ind_transition s (event l) s' p.(iolts).(sc_lts).(lts)) ->
+      ind_out_one_state s so p.
 
-Definition ind_ioco (i s : s_IOLTS) : Prop := 
+Definition ind_out (Q : set state) (so : set out_label) (p : s_IOLTS) : Prop :=
+  forall (x : out_label),
+    In x so <->
+    exists (s : state) (so' : set out_label),
+      (In s Q /\ ind_out_one_state s so' p /\ In x so').
+
+Lemma out_label_dec :
+  forall (o1 o2 : out_label), {o1 = o2} + {o1 <> o2}.
+Proof.
+  decide equality. apply string_dec.
+Qed.
+
+Fixpoint f_out_one_state' (s : state) (lt: list transition) (Lu : set label)
+    : set out_label :=
+  match lt with
+  | [] => []
+  | (q1, e, q2) :: t =>
+      if s =? q1
+      then
+        match e with
+        | event e' =>
+            if set_mem string_dec e' Lu
+            then set_add out_label_dec (out_event e') (f_out_one_state' s t Lu)
+            else f_out_one_state' s t Lu
+        | tau => f_out_one_state' s t Lu
+        end
+     else f_out_one_state' s t Lu
+  end.
+
+Definition f_out_one_state (s : state) (p : s_IOLTS) : set out_label :=
+  f_out_one_state' s p.(iolts).(sc_lts).(lts).(T) p.(iolts).(L_u).
+
+Fixpoint f_out (ls : set state) (p : s_IOLTS) : set out_label :=
+  match ls with
+  | []     => []
+  | h :: t =>
+      if set_mem Nat.eq_dec h p.(Ts)
+      then set_add out_label_dec delta (f_out t p)
+      else set_union out_label_dec (f_out_one_state h p) (f_out t p)
+  end.
+
+Definition ind_ioco (i : IOTS) (s : IOLTS) : Prop :=
   forall (t : list label),
-    ind_s_traces_LTS t s ->
-      incl (f_out (f_after i.(s_iolts).(lts).(q0) t i.(T_del)) i)
-           (f_out (f_after s.(s_iolts).(lts).(q0) t s.(T_del)) s).
+    ind_s_traces_LTS t (create_s_IOLTS s) ->
+      incl (f_out
+            (f_after_LTS t i.(embedded_iolts).(sc_lts).(lts))
+            (create_s_IOLTS i.(embedded_iolts)))
+           (f_out (f_after_LTS t s.(sc_lts).(lts)) (create_s_IOLTS s)).
 
-*)
