src/IOTS.v
@@ -1,4 +1,5 @@
 Require Import LTS.
+Require Import list_helper.
 Require Import Coq.Lists.List.
 Require Import Coq.Lists.ListSet.
 Import Coq.Lists.List.ListNotations.
@@ -16,11 +17,11 @@ Section SectionIOLTS.
     Forall (fun x => ~ In x L_u) L_i.
 
   Record IOLTS : Type := mkIOLTS {
-      lts : LTS
+      sc_lts : SC_LTS
     ; L_i : list label
     ; L_u : list label
     ; disjoint_input_output_labels  : is_disjoint L_i L_u
-    ; is_IOLTS                      : (L_i ++ L_u) = lts.(L)
+    ; is_IOLTS                      : (L_i ++ L_u) [=] sc_lts.(lts).(L)
     ; no_repetition_L_i             : NoDup L_i
     ; no_repetition_L_u             : NoDup L_u
   }.
@@ -34,31 +35,17 @@ Section SectionIOLTS.
     - left. auto.
   Qed.
 
-  Lemma NoDup_dec :
-    forall {A : Type} (l : list A),
-    (forall a1 a2 : A, { a1 = a2 } + { a1 <> a2 }) ->
-     { NoDup l } + { ~ NoDup l }.
-  Proof.
-    intros A l Aeq_dec. induction l as [| h l' H].
-    - left. apply NoDup_nil.
-    - inversion H.
-      + pose proof (in_dec Aeq_dec h l') as H'. inversion H'.
-        * right. intros H''. inversion H''. auto.
-        * left. apply NoDup_cons; auto.
-      + right. intros H'. inversion H'. auto.
-  Qed.
-
-  Definition create_IOLTS (lts : LTS) (Li Lu : list label) : option IOLTS :=
+  Definition create_IOLTS (sc_lts : SC_LTS) (Li Lu : list label) : option IOLTS :=
     match is_disjoint_dec Li Lu with
     | left h_is_disjoint =>
-        match list_eq_dec string_dec (Li ++ Lu) lts.(L) with
+        match Equiv_dec (Li ++ Lu) sc_lts.(lts).(L) string_dec with
         | left h_is_IOLTS =>
             match NoDup_dec Li string_dec with
             | left h_NoDup_Li =>
                 match NoDup_dec Lu string_dec with
                 | left h_NoDup_Lu =>
                     Some (mkIOLTS
-                            lts
+                            sc_lts
                             Li
                             Lu
                             h_is_disjoint
@@ -75,13 +62,13 @@ Section SectionIOLTS.
     end.
 
   Theorem create_IOLTS_correct :
-    forall (lts : LTS) (L_i L_u : list label),
-      is_disjoint L_i L_u /\ (L_i ++ L_u) = lts.(L) /\ NoDup L_i /\ NoDup L_u
-      -> create_IOLTS lts L_i L_u <> None.
+    forall (sc_lts : SC_LTS) (L_i L_u : list label),
+      is_disjoint L_i L_u /\ (L_i ++ L_u) [=] sc_lts.(lts).(L) /\ NoDup L_i /\ NoDup L_u
+      -> create_IOLTS sc_lts L_i L_u <> None.
   Proof.
-    intros lts Li Lu H. destruct H as [H [H2 [H3 H4]]].
+    intros sc_lts Li Lu H. destruct H as [H [H2 [H3 H4]]].
     unfold create_IOLTS. destruct (is_disjoint_dec Li Lu);auto.
-    destruct (list_eq_dec string_dec (Li ++ Lu) lts.(L));auto.
+    destruct (Equiv_dec (Li ++ Lu) sc_lts.(lts).(L) string_dec);auto.
     destruct (NoDup_dec Li string_dec);auto.
     destruct (NoDup_dec Lu string_dec);auto.
     unfold not. intros H5. inversion H5.
@@ -109,8 +96,8 @@ Section SectionIOTS.
 
   Definition valid_iots (p : IOLTS) : Prop :=
       exists (ls : set state),
-          ind_der_LTS ls p.(lts) /\
-          every_elem_reaches_some_other ls p.(L_i) p.(lts).
+          ind_der_LTS ls p.(sc_lts).(lts) /\
+          every_elem_reaches_some_other ls p.(L_i) p.(sc_lts).(lts).
 
   Record IOTS : Type := mkIOTS {
       embedded_iolts                   : IOLTS
@@ -131,38 +118,28 @@ Inductive ind_quiescent : state -> IOLTS -> Prop :=
 | quiescent_r1 : forall (s : state) (p : IOLTS),
               (forall (s' : state) (l : label),
                   In l p.(L_u) ->
-                  ~ ind_transition s (event l) s' p.(lts))->
+                  ~ ind_transition s (event l) s' p.(sc_lts).(lts))->
                   (forall (s' : state),
-                  ~ ind_transition s tau s' p.(lts)) -> ind_quiescent s p.
+                  ~ ind_transition s tau s' p.(sc_lts).(lts)) -> ind_quiescent s p.
 
 Inductive ind_quiescent_traces : list label -> IOLTS -> Prop :=
 | quiescent_trace_r1  : forall (ll : list label) (p : IOLTS) (ls : set state),
-                ind_traces_LTS ll p.(lts) /\
-                    ind_after_LTS ll ls p.(lts) /\
+                ind_traces_LTS ll p.(sc_lts).(lts) /\
+                    ind_after_LTS ll ls p.(sc_lts).(lts) /\
                         (exists (s : state), In s ls /\ 
                             ind_quiescent s p) ->  ind_quiescent_traces ll p.
 
 (* Definição 9*)
 Section SectionSuspensionIOLTS.
 
-  Inductive delta_label : Type :=
-  | delta : delta_label.
-
-  (*Definition delta := "delta".*)
-
   Record s_IOLTS : Type := mksIOLTS {
-      iolts               : IOLTS
-    ; Ts                  :  list (state)
-    (*; Q_del                 :=  iolts.(lts).(Q)*)
-    (*; L_del                 :=  set_union string_dec s_iolts.(lts).(L) [delta]*)
-    (*; Li_del                :=  s_iolts.(L_i)*)
-    (*; Lu_del                :=  set_union string_dec s_iolts.(L_u) [delta]*)
-    (*; T_del                 :=  s_iolts.(lts).(T) ++ Ts*)
-    (*; delta_not_in_L        : ~ In delta s_iolts.(lts).(L)*)
-    ; valid_del_transitions : forall (s : state), 
-                                        In s Ts -> In s iolts.(lts).(Q)
-    ; Ts_complete_correct   : forall (s : state), In s Ts <-> In s iolts.(lts).(Q) /\
-                                        ind_quiescent s iolts
+      iolts : IOLTS
+    ; Ts : set state
+    ; valid_del_transitions : forall (s : state),
+                                        In s Ts -> In s iolts.(sc_lts).(lts).(Q)
+    ; Ts_complete_correct :
+        forall (s : state),
+          In s Ts <-> In s iolts.(sc_lts).(lts).(Q) /\ ind_quiescent s iolts
   }.
 
   Definition out_transition (q : state) (Lu : set label)
@@ -183,31 +160,19 @@ Section SectionSuspensionIOLTS.
     negb (existsb (out_transition q Lu) l).
 
   Definition create_Ts (iolts : IOLTS) : list state :=
-    filter (is_quiescent iolts.(lts).(T) iolts.(L_u)) iolts.(lts).(Q).
+    filter (is_quiescent iolts.(sc_lts).(lts).(T) iolts.(L_u)) iolts.(sc_lts).(lts).(Q).
 
   Lemma create_Ts_valid_del_transitions :
-    forall (iolts : IOLTS) (s : state), In s (create_Ts iolts) -> In s iolts.(lts).(Q).
+    forall (iolts : IOLTS) (s : state),
+      In s (create_Ts iolts) -> In s iolts.(sc_lts).(lts).(Q).
   Proof.
     intros iolts s H. unfold create_Ts in H. apply filter_In in H.
     destruct H as [H _]. apply H.
   Qed.
 
-  Lemma existsb_false:
-    forall (A : Type) (f : A -> bool) (l : list A),
-      existsb f l = false <-> ~ exists x : A, In x l /\ f x = true.
-  Proof.
-    intros. split.
-    - intros H. pose proof (existsb_exists f l) as H'. apply iff_sym in H'.
-      apply Bool.iff_reflect in H'. rewrite H in H'. inversion H'. auto.
-    - intros H. pose proof (existsb_exists f l) as H'. apply iff_sym in H'.
-      apply Bool.iff_reflect in H'. inversion H'.
-      + unfold not in H. destruct H. apply H1.
-      + reflexivity.
-  Qed.
-
   Lemma create_Ts_complete_correct :
     forall (iolts : IOLTS) (s : state), 
-      In s (create_Ts iolts) <-> In s iolts.(lts).(Q) /\ ind_quiescent s iolts.
+      In s (create_Ts iolts) <-> In s iolts.(sc_lts).(lts).(Q) /\ ind_quiescent s iolts.
   Proof.
     intros iolts s. split.
     - intros H. split.
@@ -253,8 +218,8 @@ End SectionSuspensionIOLTS.
 
 Inductive ind_s_traces : state -> list label -> s_IOLTS -> Prop :=
 | s_traces_r1 : forall (s : state) (t : list label) (p : s_IOLTS),
-                   ind_traces s t p.(iolts).(lts) -> ind_s_traces s t p.
+                   ind_traces s t p.(iolts).(sc_lts).(lts) -> ind_s_traces s t p.
 
 Inductive ind_s_traces_LTS : list label -> s_IOLTS -> Prop :=
 | s_traces_LTS_r1 : forall (t : list label) (p : s_IOLTS),
-                   ind_traces_LTS t p.(iolts).(lts) -> ind_s_traces_LTS t p.
+                   ind_traces_LTS t p.(iolts).(sc_lts).(lts) -> ind_s_traces_LTS t p.
